some more fixing of things

src/chapter4.lean
@@ -4,12 +4,55 @@ open chapter3
 
 namespace chapter4
 
+  -----------------------------------------------------------------------------------
+
+  def is_elem : char → 𝕋' → Prop
+  | x (#y) := y = x
+  | x ▢ := false
+  | x (t◦u) := is_elem x t ∨ is_elem x u
+
+  instance elem_decidable {x} {t} : decidable (is_elem x t) := begin
+    induction t,
+    case node {
+      left,
+      intro h,
+      cases h,
+    },
+    case app : t₁ t₂ h₁ h₂ {
+      cases h₁,
+        cases h₂,
+          left,
+          intro h,
+          cases h,
+          apply h₁,
+          assumption,
+          apply h₂,
+          assumption,
+        right,
+        right,
+        assumption,
+      cases h₂,
+        right,
+        left,
+        assumption,
+      right,
+      right,
+      assumption,
+    },
+    case ref {
+      rw is_elem,
+      exact eq.decidable t x,
+    },
+  end
+
+  -----------------------------------------------------------------------------------
+
   def subst' : char → 𝕋' → 𝕋' → 𝕋'
   | x u (#y) := if y = x then u else #y
   | x u ▢ := ▢
   | x u (s◦t) := (subst' x u s) ◦ (subst' x u t)
 
-  lemma subst_red_t {x} {u t₁ t₂} (h : t₁ ↦ t₂) : subst' x u t₁ ≈ subst' x u t₂ := begin
+  lemma subst'_red_t {x} {u t₁ t₂} (h : t₁ ↦ t₂) : subst' x u t₁ ≈ subst' x u t₂ := begin
     apply eqv_gen.rel,
     induction h,
     case kernel : y' z' {
@@ -46,7 +89,7 @@ namespace chapter4
     },
   end
 
-  lemma subst_red_u {x} {u₁ u₂ t} (h : u₁ ↦ u₂) : subst' x u₁ t ≈ subst' x u₂ t := begin
+  lemma subst'_red_u {x} {u₁ u₂ t} (h : u₁ ↦ u₂) : subst' x u₁ t ≈ subst' x u₂ t := begin
     induction t,
     case node {
       reflexivity,
@@ -67,7 +110,7 @@ namespace chapter4
     }
   end
   
-  def subst1 : char → 𝕋' → 𝕋 → 𝕋 := λ x u, quotient.lift (λ t, ⟦subst' x u t⟧) 
+  def subst'1 : char → 𝕋' → 𝕋 → 𝕋 := λ x u, quotient.lift (λ t, ⟦subst' x u t⟧) 
   ( begin
       intros a b h,
       simp,
@@ -85,13 +128,45 @@ namespace chapter4
         assumption,
       },
       case rel {
-        apply subst_red_t,
+        apply subst'_red_t,
         assumption,
       },
     end
   )
 
-  def subst : char → 𝕋 → 𝕋 → 𝕋 := λ x, quotient.lift (λ u, subst1 x u) 
+  lemma subst'_id {x} {u t} (h : ¬ is_elem x t) : subst' x u t = t := begin
+    induction t,
+    refl,
+    case app : v w hv hw {
+      rw subst',
+      apply congr_arg2,
+
+      apply hv,
+      intro p,
+      apply h,
+      rw is_elem,
+      left,
+      assumption,
+
+      apply hw,
+      intro p,
+      apply h,
+      rw is_elem,
+      right,
+      assumption,
+    },
+    rw subst',
+    split_ifs,
+    exfalso,
+    apply h,
+    rw h_1,
+    rw is_elem,
+    refl,
+  end
+
+  -----------------------------------------------------------------------------------
+
+  def subst : char → 𝕋 → 𝕋 → 𝕋 := λ x, quotient.lift (λ u, subst'1 x u) 
   ( begin
       intros a b h,
       simp,
@@ -111,11 +186,11 @@ namespace chapter4
         assumption,
       },
       case rel : u₁ u₂ h {
-        rw subst1,
+        rw subst'1,
         simp,
         have h₁ := quotient.exists_rep t, cases h₁ with t' h₁, rw ←h₁,
         simp,
-        apply subst_red_u,
+        apply subst'_red_u,
         assumption,
       }
     end
@@ -129,7 +204,7 @@ namespace chapter4
 
     rw [subst, h],
     simp,
-    rw subst1,
+    rw subst'1,
     simp,
     rw subst',
     split_ifs,
@@ -138,7 +213,7 @@ namespace chapter4
 
     rw [subst],
     simp,
-    rw subst1,
+    rw subst'1,
     simp,
     rw subst',
     split_ifs,
@@ -155,7 +230,7 @@ namespace chapter4
     rw natree.node,
     rw subst,
     simp,
-    rw subst1,
+    rw subst'1,
     simp,
     refl,
   end
@@ -166,14 +241,21 @@ namespace chapter4
     have h₃ := quotient.exists_rep (t), cases h₃ with t' h₃, rw ←h₃,
     rw subst,
     simp,
-    rw subst1,
+    rw subst'1,
     simp,
     refl,
   end
 
-  --lemma which knows that substituting into a term with no free variables of a specific character is pointless
-
-  --lemma which know that there *will* be no free 'x' variables in a term which starts with "λ* x, ..."
+  lemma subst_id {x} {u} {t} (h : ¬ is_elem x t) : subst x u ⟦t⟧ = ⟦t⟧ := begin
+    have h₁ := quotient.exists_rep u, cases h₁ with u' h₁, rw ←h₁,
+    rw subst,
+    dsimp,
+    rw subst'1,
+    dsimp,
+    apply quotient.sound,
+    rw subst'_id,
+    assumption,
+  end
 
   -----------------------------------------------------------------------------------
 
@@ -242,7 +324,7 @@ namespace chapter4
   | x (#y) := if y =  x then I' else K'◦(#y)
   | x ▢ := K'◦▢
   | x (u◦v) := (d' (bracket x v))◦(bracket x u)
-  lemma bracket_prop {x} {t} : (bracket x t)◦(# x) ≈ t := begin
+  lemma bracket_prop {x} {t} : (bracket x t)◦(#x) ≈ t := begin
     induction t,
     case node {
       rw bracket,
@@ -290,64 +372,17 @@ namespace chapter4
 
   -----------------------------------------------------------------------------------
 
-  def is_elem : char → 𝕋' → Prop
-  | x (#y) := y =  x
-  | x ▢ := false
-  | x (t◦u) := is_elem x t ∨ is_elem x u
-
-  instance elem_decidable {x} {t} : decidable (is_elem x t) := begin
-    induction t,
-    case node {
-      left,
-      intro h,
-      cases h,
-    },
-    case app : t₁ t₂ h₁ h₂ {
-      cases h₁,
-        cases h₂,
-          left,
-          intro h,
-          cases h,
-          apply h₁,
-          assumption,
-          apply h₂,
-          assumption,
-        right,
-        right,
-        assumption,
-      cases h₂,
-        right,
-        left,
-        assumption,
-      right,
-      right,
-      assumption,
-    },
-    case ref {
-      rw is_elem,
-      exact eq.decidable t ( x),
-    },
-  end
-
-  lemma is_elem_id {x} : is_elem x (# x) := by rw is_elem
-
-  -----------------------------------------------------------------------------------
-
   --star abs similarly not liftable
-  def star_abs' : char → 𝕋' → 𝕋'
+  def star_abs : char → 𝕋' → 𝕋'
   | x ▢ := K'◦▢
   | x (#y) := if is_elem x (#y) then I' else K'◦(#y)
-  | x (t◦(#y)) := if is_elem x (#y) ∧ ¬ is_elem x t then t else (d' (star_abs' x (#y)))◦(star_abs' x t) --special case for eta-reduction
-  | x (t◦u) := (d' (star_abs' x u))◦(star_abs' x t)
+  | x (t◦(#y)) := if is_elem x (#y) ∧ ¬ is_elem x t then t else (d' (star_abs x (#y)))◦(star_abs x t) --special case for eta-reduction
+  | x (t◦u) := (d' (star_abs x u))◦(star_abs x t)
 
-  notation `λ** ` x `, ` t := star_abs' x t
-
-  def star_abs (x) (t) := ⟦λ** x, t⟧ -- <-- is this actually useful??
-  
   notation `λ* ` x `, ` t := star_abs x t
 
-  lemma star_eta' {x} {t} (h : ¬ is_elem x t) : (λ** x, t◦#x) ≈ t := begin
-    rw star_abs',
+  lemma star_eta {x} {t} (h : ¬ is_elem x t) : (λ* x, t◦#x) ≈ t := begin
+    rw star_abs,
     split_ifs,
     refl,
     exfalso,
@@ -360,16 +395,16 @@ namespace chapter4
     assumption,
   end
 
-  lemma star_unchanged' {x} {t u} (h : ¬ is_elem x t) : (λ** x, t)◦u ≈ t := begin
+  lemma star_unchanged {x} {t u} (h : ¬ is_elem x t) : (λ* x, t)◦u ≈ t := begin
     induction t,
     case node {
-      rw star_abs',
+      rw star_abs,
       apply K'_prop,
     },
     case app : t₁ t₂ h₁ h₂ {
       induction t₂,
       case node {
-        rw star_abs',
+        rw star_abs,
         transitivity,
         apply d'_prop,
         apply natree.pre.equiv.congr,
@@ -381,11 +416,11 @@ namespace chapter4
         left,
         assumption,
 
-        rw star_abs',
+        rw star_abs,
         apply K'_prop,
       },
       case app : t₃ t₄ h₃ h₄ {
-        rw star_abs',
+        rw star_abs,
         transitivity,
         apply d'_prop,
         apply natree.pre.equiv.congr,
@@ -427,7 +462,7 @@ namespace chapter4
 
         symmetry,
 
-        repeat {rw star_abs'},
+        repeat {rw star_abs},
         split_ifs,
 
         exfalso,
@@ -451,20 +486,20 @@ namespace chapter4
       },
     },
     case ref {
-      rw star_abs',
+      rw star_abs,
       split_ifs,
       apply K'_prop,
     },
   end
 
-  theorem star_beta' {x} {t u} : (λ** x, t)◦u ≈ subst' x u t := begin
+  theorem star_beta {x} {t u} : (λ* x, t)◦u ≈ subst' x u t := begin
     induction t,
     case node {
-      rw [star_abs', subst'],
+      rw [star_abs, subst'],
       apply K'_prop,
     },
     case ref {
-      rw [star_abs', subst'],
+      rw [star_abs, subst'],
       split_ifs,
       apply I'_prop,
       apply K'_prop,
@@ -483,26 +518,26 @@ namespace chapter4
 
       induction t₂,
       case node {
-        rw star_abs',
+        rw star_abs,
         transitivity,
         apply d'_prop,
         refl,
       },
       case app {
-        rw star_abs',
+        rw star_abs,
         transitivity,
         apply d'_prop,
         refl,
       },
       case ref {
         repeat {
-          rw star_abs',
+          rw star_abs,
         },
         symmetry,
         split_ifs,
 
         apply natree.pre.equiv.congr,
-        apply star_unchanged',
+        apply star_unchanged,
         exact h_1.2,
         apply I'_prop,
 
@@ -520,13 +555,20 @@ namespace chapter4
     },
   end
 
-  theorem star_beta {x} {t} {u} : (λ* x, t)⬝u = subst x u ⟦t⟧ := begin
-    have h₁ := quotient.exists_rep y, cases h₁ with y' h₁, rw ←h₁,
+  theorem star_beta_q {x} {t} {u} : ⟦λ* x, t⟧⬝u = subst x u ⟦t⟧ := begin
+    have h₁ := quotient.exists_rep u, cases h₁ with u' h₁, rw ←h₁,
+    rw ←natree.quot_dist_app,
+    rw subst,
+    dsimp,
+    rw subst'1,
+    dsimp,
+    apply quotient.sound,
+    apply star_beta,
   end
 
   -----------------------------------------------------------------------------------
 
-  def ω : 𝕋 := ⟦λ** 'z', λ** 'f', #'f'◦(#'z'◦#'z'◦#'f')⟧
+  def ω : 𝕋 := ⟦λ* 'z', λ* 'f', #'f'◦(#'z'◦#'z'◦#'f')⟧
 
   def Y (f) := ω⬝ω⬝f
   lemma Y_prop {f} : Y f = f⬝(Y f) := begin
@@ -538,34 +580,41 @@ namespace chapter4
     rw ω,
     refl, refl,
 
-    have h₁ := quotient.exists_rep ω, cases h₁ with ω' h₁, rw ←h₁,
-    have h₂ := quotient.exists_rep f, cases h₂ with f' h₂, rw ←h₂,
-    repeat {rw ←natree.quot_dist_app},
-    apply quotient.sound,
-
     transitivity,
-    apply natree.pre.equiv.congr,
-    apply star_beta',
+    apply congr_arg2,
+    rw star_beta_q,
     refl,
 
-    transitivity,
-    rw star_abs',
-    rw subst',
+    --...
 
-    transitivity,
-    apply natree.pre.equiv.congr_left,
-    apply natree.pre.equiv.congr,
+    -- have h₁ := quotient.exists_rep ω, cases h₁ with ω' h₁, rw ←h₁,
+    -- have h₂ := quotient.exists_rep f, cases h₂ with f' h₂, rw ←h₂,
+    -- repeat {rw ←natree.quot_dist_app},
+    -- apply quotient.sound,
 
-    show subst' 'z' ω' (d' (λ** 'f', #'z'◦#'z'◦#'f')) ≈ d' (ω'◦ω'),
-    refl,
-    show subst' 'z' ω' (λ** 'f', #'f') ≈ I',
-    refl,
+    -- transitivity,
+    -- apply natree.pre.equiv.congr,
+    -- apply star_beta,
+    -- refl,
 
-    transitivity,
-    apply d'_prop,
+    -- transitivity,
+    -- rw star_abs,
+    -- rw subst',
 
-    apply natree.pre.equiv.congr_left,
-    apply I'_prop,
+    -- transitivity,
+    -- apply natree.pre.equiv.congr_left,
+    -- apply natree.pre.equiv.congr,
+
+    -- show subst' 'z' ω' (d' (λ* 'f', #'z'◦#'z'◦#'f')) ≈ d' (ω'◦ω'),
+    -- refl,
+    -- show subst' 'z' ω' (λ* 'f', #'f') ≈ I',
+    -- refl,
+
+    -- transitivity,
+    -- apply d'_prop,
+
+    -- apply natree.pre.equiv.congr_left,
+    -- apply I'_prop,
   end
 
   def wait (x y) := (d I)⬝((d (K⬝y))⬝(K⬝x))
@@ -588,12 +637,12 @@ namespace chapter4
   theorem fixpoint_function {f x} : (Y₂ f)⬝x = f⬝x⬝(Y₂ f) := by simp [Y₂, Z, swap, wait1, self_apply, d, D, I, K]
   lemma Y₂_prop {f x} : (Y₂ f)⬝x = f⬝x⬝(Y₂ f) := fixpoint_function
 
-  def plus : 𝕋 := Y₂ ⟦λ** 'm', λ** 'p', ▢◦#'m'◦I'◦(K'◦(λ** 'x', λ** 'n', K'◦(#'p'◦#'x'◦#'n')))⟧
+  def plus : 𝕋 := Y₂ ⟦λ* 'm', λ* 'p', ▢◦#'m'◦I'◦(K'◦(λ* 'x', λ* 'n', K'◦(#'p'◦#'x'◦#'n')))⟧
 
   def t_nil := △
   def t_cons (h t) := △⬝h⬝t
 
-  def t_head := ⟦λ** 'x', (((▢◦#'x')◦(K'◦I'))◦K')⟧
+  def t_head := ⟦λ* 'x', (((▢◦#'x')◦(K'◦I'))◦K')⟧
   lemma head_prop {h t} : t_head⬝(t_cons h t) = h := begin
     rw [t_head, t_cons],
     have h₁ := quotient.exists_rep h, cases h₁ with h' h₁, rw ←h₁,
@@ -602,7 +651,7 @@ namespace chapter4
     repeat {rw ←quot_dist_app},
     apply quotient.sound,
     transitivity,
-    apply star_beta',
+    apply star_beta,
     repeat {rw subst'},
     show (▢◦(▢◦h'◦t')◦(K'◦I')◦K') ≈ h',
     transitivity,
@@ -611,7 +660,7 @@ namespace chapter4
     apply K'_prop,
   end
 
-  def t_tail := ⟦λ** 'x', (((▢◦#'x')◦(K'◦I'))◦(K'◦I'))⟧
+  def t_tail := ⟦λ* 'x', (((▢◦#'x')◦(K'◦I'))◦(K'◦I'))⟧
   lemma tail_prop {h t} : t_tail⬝(t_cons h t) = t := begin
     rw [t_tail, t_cons],
     have h₁ := quotient.exists_rep h, cases h₁ with h' h₁, rw ←h₁,
@@ -620,7 +669,7 @@ namespace chapter4
     repeat {rw ←quot_dist_app},
     apply quotient.sound,
     transitivity,
-    apply star_beta',
+    apply star_beta,
     repeat {rw subst'},
     transitivity,
     apply natree.pre.equiv.congr,
@@ -645,10 +694,10 @@ namespace chapter4
   def t_nil' := ▢
   def t_cons' (h t) := ▢◦h◦t
 
-  def list_map_swap := ⟦(λ** 'x', ▢◦#'x'◦(K'◦(K'◦t_nil')))◦(λ** 'h', λ** 't', λ** 'm', λ** 'f', t_cons' (#'f'◦#'h') (#'m'◦#'f'◦#'t'))⟧
+  def list_map_swap := ⟦(λ* 'x', ▢◦#'x'◦(K'◦(K'◦t_nil')))◦(λ* 'h', λ* 't', λ* 'm', λ* 'f', t_cons' (#'f'◦#'h') (#'m'◦#'f'◦#'t'))⟧
   def list_map := swap (Y₂ list_map_swap)
   lemma list_map_prop_nil {f} : list_map⬝f⬝t_nil = t_nil := begin
-    --??? (we need to stop having to delve under the quotient whenever something is defined using star_abs')
+    --??? (we need to stop having to delve under the quotient whenever something is defined using star_abs)
     --if a 𝕋' has no free variables, it is a combinator, and can be turned into an expression with no variables at all, which can then be simped
     rw [list_map, list_map_swap],
 
